pcuic/theories/PCUICWeakeningEnv.v
@@ -634,7 +634,14 @@ Proof.
       ++ eapply weakening_env_conv; eauto.
       ++ eapply weakening_env_cumul; eauto.
   - red in onP |- *. eapply All_local_env_impl; eauto.
-Qed.
+  - move: onVariance.
+    rewrite /on_variance. destruct ind_universes => //.
+    destruct ind_variance => //.
+    intros [univs' [i [i' []]]]. exists univs', i, i'. split => //.
+    2-3:eapply weakening_env_consistent_instance; tea.
+    split.
+    all:admit.  
+Admitted.
 
 Lemma weakening_env_lookup_on_global_env `{checker_flags} P Σ Σ' c decl :
   weaken_env_prop P ->
